

assume P true for all  $k \leq n$  for some  $n > 1$

Inductive  $F(n)$  is even IFF  $F(n+3)$  is even  
Hypothesis:  
Base case:  $F(0) = 0$   $F(3) = 2$  both even ✓  
 $F(1) = 1$   $F(4) = 3$  both not even ✓  
Induction step:  
• Assume P(n) true for  $0 \leq n \leq k$   
WTS true for  $n = k+1$   
 $n = \frac{k+1}{2}$  are true WTS true for  $n = k+1$

•  $F(n+1)$  is even IFF  $F(n) + F(n-1)$  is even  
•  $F(n) + F(n-1)$  is even IFF  $F(n)$  and  $F(n-1)$  are both even or odd. [sums addition]  
 $F(n)$  even  $\leftrightarrow F(n+3)$  even  $F(n-1)$  even  $\leftrightarrow F(n+2)$  even  
even  $\leftrightarrow$  even  
Even + Even = Even  
Odd + odd = Even  
Even + odd = odd

$$\therefore F(n+4) = F(n+3) + F(n+2)$$

even  $\leftrightarrow$  even  
Even + Even = Even  
Odd + odd = Even  
Even + odd = odd

$F(n+1)$  even IFF  $F(n) \neq F(n-1)$  are both even or both odd  
Same even/odd pairs by assumption  
 $F(n+4)$  even IFF  $F(n+3) \neq F(n+2)$  are both even or both odd  
 $F(n+1)$  is even IFF  $F(n+4)$  is even. ....

Total value of annuity

$$0 \quad V = \sum_{i=1}^n \frac{M}{(1+r)^i} = M \sum_{i=1}^n \left(\frac{1}{1+r}\right)^i = M \left(\frac{1}{1+r}\right) \frac{1 - \left(\frac{1}{1+r}\right)^{n+1}}{1 - \frac{1}{1+r}} = M \frac{1 - \frac{1}{(1+r)^{n+1}}}{r}$$

$$\sum_{i=1}^{\infty} \frac{1}{1+r} = \frac{1}{r} \quad r = \frac{1}{(1+r)}$$

$$0 \quad \sum_{k=1}^n k^2 = 1^2 + 2^2 + 3^2 + \dots + n^2 = \frac{n(n+1)(2n+1)}{6}$$

$$0 \quad \sum_{k=1}^n k = 1 + 2 + 3 + \dots + n = \frac{n(n+1)}{2}$$

$$0 \quad \sum_{i=0}^{n-1} ar^i = a + ar + ar^2 + \dots + ar^{n-1} = a \frac{r^n - 1}{r - 1} \rightarrow a \text{ can be } 1$$

$$0 \quad \sum_{i=1}^n r^i = r \left( \frac{r^n - 1}{r - 1} \right)$$

$$0 \quad \sum_{k=1}^n kx^k = \frac{x + x^{n+1}(nx - n - 1)}{(1-x)^2}$$

(b) [5 pts] Use the perturbation method to find a closed-form expression for  $S = \sum_{k=1}^{\infty} k^2 3^k$ .  
Hint: Perturb once, then use the formula listed above.

Solution. We perturb once to get

$$3S = 3 \sum_{k=1}^{\infty} k^2 3^k = \sum_{k=1}^{\infty} k^2 3^{k+1}$$

We now subtract 3S from S:

$$S - 3S = 1^2 \cdot 3^1 + 2^2 \cdot 3^2 + 3^2 \cdot 3^3 + \dots + n^2 \cdot 3^n - 1^2 \cdot 3^2 - 2^2 \cdot 3^3 - \dots - (n-1)^2 \cdot 3^n - n^2 \cdot 3^{n+1}$$

which becomes

$$S - 3S = 1^2 \cdot 3^1 - n \cdot 3^{n+1} + \sum_{k=2}^n (k^2 - (k-1)^2) 3^k$$

$$= 3 - n^2 \cdot 3^{n+1} + \sum_{k=2}^n (2k-1) 3^k$$

$$= 3 - n^2 \cdot 3^{n+1} + 2 \sum_{k=2}^n k 3^k - \sum_{k=2}^n 3^k$$

$$= 3 - n^2 \cdot 3^{n+1} + 2 \left( \frac{3(n \cdot 3^{n+1} - (n+1)3^n + 1)}{(3-1)^2} \right) - 3 \left( \frac{3^n - 1}{3-1} - 3 \right)$$

$$= 3 - n^2 \cdot 3^{n+1} + \frac{3}{2} (2n \cdot 3^n - 3^n - 3) - \frac{3}{2} (3^n - 3)$$

$$= 3 - n^2 \cdot 3^{n+1} + n \cdot 3^n - 3 \cdot 3^n$$

(d) Explain why the Master Theorem cannot be used to analyze  $T(n) = 2T(\lfloor n/2 \rfloor) + n \log n$ . (You don't need to find a  $\Theta$ -bound yourself, but it could be a fun optional challenge!)

Solution. Since  $a = b = 2$ , the critical exponent is  $\log_2 a = 1$ . The ratios  $(n \log n)/n^1$  and  $n^{1/2}/(n \log n)$  both limit to  $\infty$  as  $n \rightarrow \infty$ , no matter how small  $\epsilon > 0$  is chosen, so  $f(n)$  grows too fast to belong to  $\Theta(n^1)$  (so cases 1 and 2 don't apply), and at the same time,  $f(n)$  grows too slow for  $\Omega(n^{1+\epsilon})$  (so case 3 doesn't apply).

This example shows that the Master Theorem is not exhaustive: there are cases like this one that can "fall through the cracks" by being simultaneously too big for case 2 but too small for case 3. It's possible to fit between cases 1 and 2 similarly; try to come up with such an example.

So how would we analyze this algorithm? Some options include a more detailed recursion tree analysis, or a careful induction argument. Try it yourself!

Now let  $k = \log_3 n$ . The formula then becomes

$$T(n) = 3^k T\left(\frac{n}{3^k}\right) + 2kn - \frac{3^k - 3}{2} + \frac{3}{2}$$

$$= 3^{\log_3 n} T\left(\frac{n}{3^{\log_3 n}}\right) + 2n \log_3 n - \frac{3^{\log_3 n} - 3}{2} + \frac{3}{2}$$

$$= nT(1) + 2n \log_3 n - \frac{3}{2}n + \frac{3}{2}$$

$$= 2n \log_3 n - \frac{3}{2}n + \frac{3}{2}$$

#### 5.4 Asymptotics Tips

- Something is  $\Theta$  if and only if it is  $O$  and  $\Omega$ .
- If something is  $\omega$ , then it is also  $O$ . The other way around is not for certain.
- If something is  $\omega$ , then it is also  $\Omega$ . The other way around is not for certain.
- Refer to the following order of largeness (biggest is highest up on the list, smallest is lowest on the list):
  - $O(n!)$  (factorial)
  - $O(2^n)$  or any constant raised to  $n$  (exponential)
  - $O(n^c)$  or  $n$  raised to any constant (polynomial)
  - $O(n \log n)$  (log linear)
  - $O(n)$  (linear)
  - $O(\log n)$  (log)

#### Problem 6. Recurrences

Use the Plug and Chug method to find an exact closed form formula for  $a(n)$  as a function of  $n$ , where  $a(n) = 2a(n-1) + 3^n$  for  $n \geq 1$ , and  $a(0) = 5$ .

Solution. We perform a few substitutions to look for a pattern:

$$a(n) = 3^n + 2a(n-1)$$

$$= 3^n + 2(3^{n-1} + 2a(n-2))$$

$$= 3^n + 2 \cdot 3^{n-1} + 4a(n-2)$$

$$= 3^n + 2 \cdot 3^{n-1} + 2^2 \cdot 3^{n-2} + 8 \cdot a(n-3)$$

$$\vdots$$

After  $k$  expansions, we can guess that the formula takes the form

$$a(n) = 3^n + 2 \cdot 3^{n-1} + \dots + 2^k 3^{n-k} + 2^{k+1} a(n-k-1)$$

$$= \left( \sum_{i=0}^k 2^i \cdot 3^{n-i} \right) + 2^{k+1} a(n-k-1)$$

Choosing  $k = n-1$ , we find that

$$= \left( \sum_{i=0}^{n-1} 2^i \cdot 3^{n-i} \right) + 2^n \cdot a(0)$$

$$= 3^n \cdot \frac{1 - (2/3)^n}{1 - (2/3)} + 5 \cdot 2^n$$

**Predicate**  
Contrapositive (equivalent)  
 $(x \rightarrow y) \leftrightarrow (\neg y \rightarrow \neg x)$   
Converse (not equivalent)  
 $(x \rightarrow y) \rightarrow (y \rightarrow x)$   
SETS  
 $A = \{6, 1, 3, 0\}$   $\mathbb{N} \subseteq A$  ✓  
 $\{3\} \subseteq A$  ✓  
 $\{1, 2, 3\} \subseteq A$  ✓  
Set BUILDER  
 $\{n \in \mathbb{N} \mid \text{isPrime}(n)\} = \{2, 3, 5, 7, 11, \dots\}$   
 $A \cap B$  OR  $A - B = A \setminus B$   
AND  $x \in A$  AND  $x \notin B$   
NOTATION

$$1 + r + r^2 + r^3 + \dots + r^n + r^{n+1} = \frac{1 - r^{n+1}}{1 - r} + r^{n+1}$$

$$S = 1 + r + r^2 + r^3 + \dots + r^n$$

$$rS = r + r^2 + r^3 + \dots + r^{n+1}$$

$$S - rS = 1 - r^{n+1}$$

$$S = \frac{1 - r^{n+1}}{1 - r}$$

#### Problem 3. Contradiction

Prove by contradiction that if  $a \cdot b = n$ , then either  $a$  or  $b$  must be  $\leq \sqrt{n}$ , where  $a, b$ , and  $n$  are nonnegative real numbers.

Solution. Suppose to the contrary that  $a > \sqrt{n}$  and  $b > \sqrt{n}$ . Then

$$a \cdot b > \sqrt{n} \cdot \sqrt{n} = n$$

contradicting the fact that  $a \cdot b = n$ .

Here we have used the rule that for nonnegative real numbers  $u, v, w, x$ ,

$$[u > v \text{ AND } w > x] \text{ IMPLIES } u \cdot w > v \cdot x$$

This rule applies since  $a, b$ , and  $\sqrt{n}$  are nonnegative.

Note that we are using the fact that if  $n$  is nonnegative, then  $\sqrt{n}$  denotes the nonnegative square root. If we had used the negative square root of  $n$ , the above rule would not hold, and the proof would not be correct. Indeed, if we used the negative square root of 2 with  $a = b = 1$ , the claim to be proved would be false.

(b) Suppose we start with 100 of each token. Prove carefully that the state (50,8) is unreachable. If you would like to use a fact from the previous part, you must prove it here.

Solution. Define the predicate  $P(n_a, n_b) : \text{rem}(n_a + n_b, 3) = 2$ ; we'll prove that  $P$  is invariant.

At the start state (100,100), the property  $P(100,100)$  holds because  $100 + 100 = 200 \equiv 2 \pmod{3}$ . Now assume we have any state  $(n_a, n_b)$  where  $P(n_a, n_b)$  holds; we must show that  $P$  still holds after following any transition from  $(n_a, n_b)$ . The first kind of transition takes us to  $(n_a - 1, n_b + 1)$ , and  $(n_a - 1) + (n_b + 1) = n_a + n_b$ , which has remainder 2 when divided by 3 (by assumption), so the property holds. For the second kind of transition,  $(n_a + 3) + (n_b - 6) = n_a + n_b - 3$ , which has the same remainder as  $n_a + n_b$ , namely, 2. Since  $P(n_a, n_b)$  is true at the start state and is preserved across transitions, the Invariant Principle shows that it is true at all reachable states.

However (50,8) has 50 + 8, which has remainder 1, thus it is unreachable. ■

$$S = \sum_{i=1}^{\infty} \frac{1}{(2i-1)^2}$$

$$u \leq S \leq v \quad \text{and} \quad |v - u| \leq \frac{1}{100}$$

$$u = f(1) + f(3) + f(5) + f(7) + f(9) + \dots + \frac{1}{(2i-1)^2}$$

$$v = f(2) + f(4) + f(6) + f(8) + f(10) + \dots + \frac{1}{(2i-1)^2}$$

$$T(n) = 3T\left(\frac{n}{3}\right) + 2n - 3$$

$$= 3\left(3T\left(\frac{n}{9}\right) + \frac{2n}{3} - 3\right) + 2n - 3$$

$$= 9T\left(\frac{n}{9}\right) + (2n - 9) + (2n - 3)$$

$$= \dots$$

$$= 3^k T\left(\frac{n}{3^k}\right) + 2kn - (3^k + 3^{k-1} + \dots + 3)$$

$$= 3^k T\left(\frac{n}{3^k}\right) + 2kn - \frac{3(3^k - 1)}{3 - 1}$$

$$= 3^k T\left(\frac{n}{3^k}\right) + 2kn - \frac{3^k - 3}{2} + \frac{3}{2}$$

## 5 Asymptotics

### 5.1 Definitions

- Big O:**  $f(n) \in O(g(n))$  if there exists some  $n_0 \in \mathbb{N}$  and  $c > 0$  such that for all  $n \geq n_0$ , we have  $|f(n)| \leq c \cdot g(n)$ . Intuition: all functions that are "at most"  $g(n)$ .
- Big Omega:**  $f(n) \in \Omega(g(n))$  if  $g(n) \in O(f(n))$ . (We can apply the Big O definition, but with  $f$  and  $g$  swapped.) Intuition: all functions that are "at least"  $g(n)$ .

- Big Theta:**  $f(n) \in \Theta(g(n))$  if  $f \in O(g)$  and  $g \in O(f)$ . Intuition:  $f$  and  $g$  are about the same, up to constant factors.

- Little O:**  $f(n) \in o(g(n))$  precisely when  $\lim_{n \rightarrow \infty} f(n)/g(n) = 0$ . Intuition:  $f$  grows much slower than  $g$ .

- Little Omega:**  $f(n) \in \omega(g(n))$  precisely when  $g(n) \in o(f(n))$ , i.e.,  $\lim_{n \rightarrow \infty} f(n)/g(n) = \infty$ . Intuition:  $f$  grows much faster than  $g$ .

- Asymptotic Equivalence:**  $f(n) \sim g(n)$  ( $f$  and  $g$  are asymptotically equivalent) precisely when  $\lim_{n \rightarrow \infty} f(n)/g(n) = 1$ .

$$n! \sim \sqrt{2\pi n} \cdot \left(\frac{n}{e}\right)^n$$

**Theorem 1 (Master Theorem).** Let  $a \geq 1$  and  $b > 1$  be constants, let  $f(n)$  be a function, and let  $T(n)$  be defined on the nonnegative integers by the recurrence

$$T(n) = aT\left(\frac{n}{b}\right) + f(n)$$

Then  $T(n)$  has the following asymptotic bounds:

- If  $f(n) \in O(n^{(\log_b a) - \epsilon})$  for some constant  $\epsilon > 0$ , then  $T(n) \in \Theta(n^{\log_b a})$ .
- If  $f(n) \in \Theta(n^{\log_b a})$ , then  $T(n) \in \Theta(n^{\log_b a} \log n)$ .
- If  $f(n) \in \Omega(n^{(\log_b a) + \epsilon})$  for some constant  $\epsilon > 0$ , and if  $a f(\lfloor n/b \rfloor) \leq c f(n)$  for some constant  $c < 1$  and all sufficiently large  $n$ , then  $T(n) \in \Theta(f(n))$ .

This theorem is also true if we replace  $\lfloor n/b \rfloor$  with  $\lceil n/b \rceil$  everywhere.

We can model this as a state machine whose states are pairs  $(n_a, n_b)$  where  $n_a \geq 0$  equals the number of ten cent tokens, and  $n_b \geq 0$  equals the number of seven cent tokens. The allowed transitions are

$$(n_a, n_b) \rightarrow (n_a - 1, n_b + 1) \quad \text{if } n_a \geq 1, \text{ and}$$

$$(n_a, n_b) \rightarrow (n_a + 3, n_b - 6) \quad \text{if } n_b \geq 6.$$

